\documentclass[12pt]{letter}
\usepackage{babel}

\usepackage[utf8]{inputenc}
\usepackage{amsmath}

\newcommand{\ket}[1]{$\left|{#1}\right\rangle$} 
\newcommand{\bra}[1]{$\left\langle{#1}\right|$}
\newcommand{\braket}[2]{$\left\langle{#1}\middle|{#2}\right\rangle$}
\newcommand{\fract}[2]{$\frac{#1}{#2}$}

\newcommand{\matrixbraket}[2]{
	$\begin{pmatrix}
		#1 \\
		#2 \\
	\end{pmatrix}$
}

\begin{document}

%\ket{1}
%\bra{0}
%\braket{0}{1}

\ket{0} = \matrixbraket{1}{0}
	
\ket{1} = \matrixbraket{0}{1}

\textit{H}(\ket{0}) = \fract{1}{\sqrt{2}}\ket{0} + \fract{1}{\sqrt{2}}\ket{1} =: \ket{+}

\textit{H}(\ket{1}) = \fract{1}{\sqrt{2}}\ket{0} - \fract{1}{\sqrt{2}}\ket{1} =: \ket{-}

\textit{H}(\fract{1}{\sqrt{2}}\ket{0} + \fract{1}{\sqrt{2}}\ket{1}) = \fract{1}{2}(\ket{0} + \ket{1}) + \fract{1}{2}(\ket{0} - \ket{1}) = \ket{0}

\textit{H}(\fract{1}{\sqrt{2}}\ket{0} - \fract{1}{\sqrt{2}}\ket{1}) = \fract{1}{2}(\ket{0} + \ket{1}) - \fract{1}{2}(\ket{0} - \ket{1}) = \ket{1}

\end{document}